Proof repair_cr reorders

mixfix/MixfixDisambiguation.v
@@ -30,8 +30,8 @@ Record conflict_rules (T : Type) := mk_conflict_rules {
   conflict_right : production T → production T → Prop;
   conflict_left_decidable : RelDecision conflict_left;
   conflict_right_decidable : RelDecision conflict_right;
-  conflict_left_well_formed : ∀ p1 p2, conflict_left p1 p2 → left_reorderable p2 p1;
-  conflict_right_well_formed : ∀ p1 p2, conflict_right p1 p2 → left_reorderable p1 p2;
+  conflict_left_well_formed : ∀ p1 p2, conflict_left p1 p2 → left_dangling p1 ∧ right_dangling p2;
+  conflict_right_well_formed : ∀ p1 p2, conflict_right p1 p2 → right_dangling p1 ∧ left_dangling p2;
 }.
 
 Global Arguments conflict_left {_} _ _ _.
@@ -122,57 +122,63 @@ with conflict_free_forest_tree := Induction for conflict_free_forest Sort Prop.
 Inductive as_conflict_right_rule {T} (PR : drules T) : production T → production T → Prop :=
   | priority_pattern_right p1 p2 :
       p1 >> p2 ∠ PR →
-      left_reorderable p1 p2 →
+      right_dangling p1 →
+      left_dangling p2 →
       as_conflict_right_rule PR p1 p2
   | left_associativity_right p1 p2 :
       p1 lefta p2 ∠ PR →
-      left_reorderable p1 p2 →
+      right_dangling p1 →
+      left_dangling p2 →
       as_conflict_right_rule PR p1 p2.
 
 Inductive as_conflict_left_rule {T} (PR : drules T) : production T → production T → Prop :=
   | priority_pattern_left p1 p2 :
       p1 >> p2 ∠ PR →
-      left_reorderable p2 p1 →
+      left_dangling p1 →
+      right_dangling p2 →
       as_conflict_left_rule PR p1 p2
   | right_associativity_left p1 p2 :
       p1 righta p2 ∠ PR →
-      left_reorderable p2 p1 →
+      left_dangling p1 →
+      right_dangling p2 →
       as_conflict_left_rule PR p1 p2.
 
-Global Instance as_conflict_right_rule_decidable {T} (PR : drules T) :
-  RelDecision (as_conflict_right_rule PR).
+Global Instance as_conflict_right_rule_decidable {T} (PR : drules T) : RelDecision (as_conflict_right_rule PR).
 Proof.
   intros p1 p2.
-  destruct (decide (left_reorderable p1 p2)) as [Hlr|Hnlr].
-  - destruct (decide (p1 >> p2 ∠ PR)) as [Hprio|Hnprio].
-    + left. auto using priority_pattern_right.
-    + destruct (decide (p1 lefta p2 ∠ PR)) as [Hlefta|Hnlefta].
-      * left. auto using left_associativity_right.
-      * right. intro. inv H; auto.
+  destruct (decide (right_dangling p1)) as [Hrd|Hnrd].
+  - destruct (decide (left_dangling p2)) as [Hld|Hnld].
+    + destruct (decide (p1 >> p2 ∠ PR)) as [Hprio|Hnprio].
+      * left. auto using priority_pattern_right.
+      * destruct (decide (p1 lefta p2 ∠ PR)) as [Hlefta|Hnlefta].
+        **left. auto using left_associativity_right.
+        **right. intro. inv H; auto.
+    + right. intro. inv H; auto.
   - right. intro. inv H; auto.
 Qed.
 
-Global Instance as_conflict_left_rule_decidable {T} (PR : drules T) :
-  RelDecision (as_conflict_left_rule PR).
+Global Instance as_conflict_left_rule_decidable {T} (PR : drules T) : RelDecision (as_conflict_left_rule PR).
 Proof.
   intros p1 p2.
-  destruct (decide (left_reorderable p2 p1)) as [Hrl|Hnrl].
-  - destruct (decide (p1 >> p2 ∠ PR)) as [Hprio|Hnprio].
-    + left. auto using priority_pattern_left.
-    + destruct (decide (p1 righta p2 ∠ PR)) as [Hlefta|Hnlefta].
-      * left. auto using right_associativity_left.
-      * right. intro. inv H; auto.
+  destruct (decide (left_dangling p1)) as [Hld|Hnld].
+  - destruct (decide (right_dangling p2)) as [Hrd|Hnrd].
+    + destruct (decide (p1 >> p2 ∠ PR)) as [Hprio|Hnprio].
+      * left. auto using priority_pattern_left.
+      * destruct (decide (p1 righta p2 ∠ PR)) as [Hrighta|Hnrighta].
+        **left. auto using right_associativity_left.
+        **right. intro. inv H; auto.
+    + right. intro. inv H; auto.
   - right. intro. inv H; auto.
 Qed.
 
 Lemma as_conflict_right_rule_well_formed {T} (PR : drules T) :
-  ∀ p1 p2, as_conflict_right_rule PR p1 p2 → left_reorderable p1 p2.
+  ∀ p1 p2, as_conflict_right_rule PR p1 p2 → right_dangling p1 ∧ left_dangling p2.
 Proof.
   intros. inv H; auto.
 Qed.
 
 Lemma as_conflict_left_rule_well_formed {T} (PR : drules T) :
-  ∀ p1 p2, as_conflict_left_rule PR p1 p2 → left_reorderable p2 p1.
+  ∀ p1 p2, as_conflict_left_rule PR p1 p2 → left_dangling p1 ∧ right_dangling p2.
 Proof.
   intros. inv H; auto.
 Qed.
