mixfix/theorems/MixfixRepairReorder.v
@@ -1,5 +1,6 @@
 From disamb Require Export MixfixRepair.
 From disamb Require Export MixfixReorder.
+From disamb Require Import MixfixUtilsTheorems.
 From disamb Require Import MixfixReorderTheorems.
 From disamb Require Import MyUtils.
 
@@ -7,65 +8,109 @@ Section MixfixRepairReorder.
 
 Context {T : Type}.
 Implicit Types (t : parse_tree T) (ts : parse_forest T) (p : production T) (X : symbol T)
-  (g : mixfixgrammar T) (Xs : list (symbol T)) (b : bool).
+  (g : mixfixgrammar T) (Xs : list (symbol T)) (b : bool) (Q : crules T).
 
-Lemma repair_cl_reorder g Q p t1 ts t' b :
-  wft g E t1 →
-  repair_cl Q p t1 ts = (t', b) → reorder_tree (node p (cons_forest t1 ts)) t'.
+Lemma repair_cr_true_left_branching g X Q p ts tn t' :
+  wft g X tn → repair_cr Q p ts tn = (t', true) → left_branching tn.
 Proof.
-  intro Hwf. revert t' ts b. induction Hwf using well_formed_parse_tree_forest_rec
-    with (P0 := fun p1 t1s Hwfts => ∀ ts ts' b, (b = true ∨ p CL p1 ∠ Q) →
-                            repair_cl_forest Q p t1s ts = (ts', b) →
-                            reorder_tree (node p (cons_forest (node p1 t1s) ts)) (node p1 ts'));
-    intros.
-  - simpl in *. inv H. apply rtc_refl.
-  - simpl in *. destruct (repair_cl_forest Q p ts ts0) eqn:E.
-    destruct (decide (b0 = true ∨ p CL p0 ∠ Q)).
+  intros Hwft. revert t'. induction Hwft using well_formed_parse_tree_forest_rec
+    with (P0 := fun pn tns Hwfts => ∀ t', repair_cr_forest Q p pn ts tns = (t', true) →
+                                          left_branching_forest tns); simpl; intros.
+  - inv H.
+  - constructor. eauto.
+  - inv H.
+  - destruct (repair_cr Q p ts t) as [tn1' b] eqn:E.
+    destruct (decide (b = true ∨ p CR X :: Xs ∠ Q)); [|inv H].
+    destruct o.
+      + subst. assert (left_branching t); eauto.
+        inv H0. constructor.
+      + inv H. apply conflict_right_well_formed in H0. destruct H0.
+        inv H0.
+        inv Hwft.
+        constructor.
+Qed.
+
+Lemma wf_crule_node g X Xs Q p tn p1 :
+  wft g X tn → p1 CR X :: Xs ∠ Q → X = E.
+Proof.
+  intros Hwft Hcrule.
+  inv Hwft; auto.
+  apply conflict_right_well_formed in Hcrule.
+  destruct Hcrule.
+  inv H0.
+Qed.
+
+Lemma repair_cr_conflict_node g X Q p ts tn t' b p1 Xs :
+  wft g X tn → repair_cr Q p ts tn = (t', b) → (b = true ∨ p1 CR X :: Xs ∠ Q) → X = E.
+Proof.
+  intros.
+  destruct H1.
+  - subst.
+    eapply repair_cr_true_left_branching in H0; eauto.
+    inv H0.
+    inv H.
+    reflexivity.
+  - eauto using wf_crule_node.
+Qed.
+
+Lemma repair_cr_reorder g X Q p ts tn t' b :
+  wft g X tn → repair_cr Q p ts tn = (t', b) → reorder_tree (node p (add_last ts tn)) t'.
+Proof.
+  intro Hwft.
+  revert t' b.
+  induction Hwft using well_formed_parse_tree_forest_rec
+    with (P0 := fun pn tns Hwfts => ∀ t' b, repair_cr_forest Q p pn ts tns = (t', b) →
+                                            reorder_tree (node p (add_last ts (node pn tns))) t'); intros.
+  - inv H. apply rtc_refl.
+  - eauto.
+  - inv H. apply rtc_refl.
+  - simpl in H.
+    destruct (repair_cr Q p ts t) eqn:E.
+    destruct (decide (b0 = true ∨ p CR X :: Xs ∠ Q)).
     + inv H.
-      eapply IHHwf; eauto.
-    + inv H. apply rtc_refl.
-  - simpl in *. exfalso.
-    destruct H.
-    + subst. inv H0.
-    + destruct Q.
-      apply left_pattern_well_formed in H.
-      eapply left_reorderable_nil_false. eassumption.
-  - destruct ts.
-    + destruct (repair_cl Q p t ts0) eqn:F. inv H0.
-      inv w.
-      inv Hwf.
-      * exfalso.
-        simpl in F. inv F.
-        destruct H; try inv H.
-        destruct Q.
-        apply left_pattern_well_formed in H.
-        eapply left_reorder_terminal_false. eassumption.
-      * eapply rtc_l.
-        **repeat constructor.
-        **apply IHHwf in F.
-          apply reorder_forest_reorder_tree.
-          apply reorder_head_tree_reorder_forest.
-          assumption.
-    + destruct (repair_cl_forest Q p (cons_forest p0 ts) ts0) eqn:F. inv H0.
-      simpl in *.
+      assert (E' := E).
+      eapply repair_cr_conflict_node in E'; eauto.
+      subst.
+      inv Hwft.
+      rewrite <- E in IHHwft. apply IHHwft in E.
+      eapply rtc_l.
+      eapply sc_rl.
+      eapply reorder_step_add_last.
+      apply reorder_forest_reorder_tree.
+      apply reorder_head_tree_reorder_forest.
+      assumption.
+    + inv H.
+      apply rtc_refl.
+Qed.
 
-
-Lemma rcl_reorder Q t :
-  reorder_tree t (rcl Q t).
+Lemma repair_cr_start_reorder g X Q t :
+  wft g X t → reorder_tree t (repair_cr_start Q t).
 Proof.
-  induction t.
+  intro Hwft.
+  inv Hwft.
   - simpl. apply rtc_refl.
-  - simpl. destruct p0.
+  - simpl. destruct ts as [|t ts].
     + apply rtc_refl.
-    + destruct (repair_cl Q p p0 p1) eqn:E.
+    + destruct (split_last t ts) as [tsh tn] eqn:Hsplit.
+      destruct (repair_cr Q p tsh tn) as [t' b] eqn:Hrepair.
+      inv H0.
+      eapply split_last_wf in Hsplit as Htnwf; eauto.
+      destruct Htnwf as [Xn Htnwf].
+      eapply repair_cr_reorder in Hrepair; eauto.
+      erewrite split_last_add_last in Hrepair; eauto.
+Qed.
 
-
-Theorem repair_reorder Q t :
-  reorder_tree t (repair Q t).
+(* Lemma repair_cl_reorder g p t1 ts Q :
+  wft g E (node p (cons_forest t1 ts)) → reorder_tree (node p (cons_forest t1 ts)) (repair_cl Q p t1 ts).
 Proof.
-  induction t using parse_tree_forest_rec
-    with (P0 := fun ts => reorder_forest ts (repair_forest Q ts)).
-  - simpl. apply rtc_refl.
-  - cbn [repair]. destruct (repair_forest Q p0) eqn:E.
-    + simpl. apply reorder_forest_reorder_tree. assumption.
-    + 
+  intro Hwft.
+  induction t1 as [a|p1 t1s].
+  - cbn [repair_cl].
+    eapply repair_cr_start_reorder; eauto.
+  - cbn [repair_cl].
+    destruct t1s.
+    + eapply repair_cr_start_reorder; eauto.
+    + destruct (repair_cl_forest Q p p1 ts t1s) eqn:E.
+      * *)
+
+End MixfixRepairReorder.
