mixfix/theorems/MixfixUtilsTheorems.v
@@ -1,0 +1,39 @@
+From disamb Require Export MixfixUtils.
+From disamb Require Import MyUtils.
+
+Section MixfixUtilsTheorems.
+
+Context {T : Type}.
+Implicit Types (t : parse_tree T) (ts : parse_forest T) (p : production T) (X : symbol T)
+  (g : mixfixgrammar T) (Xs : list (symbol T)).
+
+Lemma split_last_wf g X t Xs ts ts1 tn :
+  wft g X t → wfts g Xs ts → split_last t ts = (ts1, tn) → ∃ Xn, wft g Xn tn.
+Proof.
+  intros Hwft Hwfts.
+  revert Hwft. revert X t ts1.
+  induction Hwfts; simpl; intros.
+  - inv H.
+    eauto.
+  - destruct (split_last t ts) eqn:E.
+    inv H0.
+    eapply IHHwfts.
+    apply H.
+    apply E.
+Qed.
+
+Lemma split_last_add_last t ts tsh tn :
+  split_last t ts = (tsh, tn) → add_last tsh tn = cons_forest t ts.
+Proof.
+  revert t tsh.
+  induction ts; simpl; intros t tsh Hsplit.
+  - inv Hsplit.
+    simpl.
+    reflexivity.
+  - destruct (split_last p ts) eqn:E.
+    inv Hsplit.
+    simpl.
+    erewrite IHts; eauto.
+Qed.
+
+End MixfixUtilsTheorems.
